rename clsf_expr to clsf_expr and clsf_lvalue to get rid of bool argument, and use it in ifc_ifthenelse to demand that the condition only depends on low data

ifc/clsf_expr.v
@@ -10,7 +10,7 @@ Definition is_array_type(t: type): bool := match t with
 
 (* Only accepts expressions without memory access -- otherwise it returns None.
    Inspired by no_loads_expr in examples/expr_test.v *)
-Fixpoint clsf_expr(N: ident -> label)(as_lvalue: bool)(e: expr): option label := match e with
+Fixpoint clsf_expr_lr(as_lvalue: bool)(N: ident -> label)(e: expr): option label := match e with
   | Econst_int _ _ => Some Lo
   | Econst_float _ _ => Some Lo
   | Econst_single _ _ => Some Lo
@@ -21,13 +21,16 @@ Fixpoint clsf_expr(N: ident -> label)(as_lvalue: bool)(e: expr): option label :=
   | Evar _ t => if as_lvalue || is_array_type t then Some Lo else None
   (* tempvar means local var, whose access is handled like a stack access *)
   | Etempvar name _ => Some (N name)
-  | Ederef e1 t => if as_lvalue then clsf_expr N true e1 else None
-  | Eaddrof e1 _ => clsf_expr N true e1
-  | Eunop _ e1 _ => clsf_expr N as_lvalue e1
-  | Ebinop _ e1 e2 _ => lub (clsf_expr N as_lvalue e1) (clsf_expr N as_lvalue e2)
-  | Ecast e1 _ => clsf_expr N as_lvalue e1
-  | Efield e1 _ t => if as_lvalue || is_array_type t then clsf_expr N true e1 else None
+  | Ederef e1 t => if as_lvalue then clsf_expr_lr true N e1 else None
+  | Eaddrof e1 _ => clsf_expr_lr true N e1
+  | Eunop _ e1 _ => clsf_expr_lr as_lvalue N e1
+  | Ebinop _ e1 e2 _ => lub (clsf_expr_lr as_lvalue N e1) (clsf_expr_lr as_lvalue N e2)
+  | Ecast e1 _ => clsf_expr_lr as_lvalue N e1
+  | Efield e1 _ t => if as_lvalue || is_array_type t then clsf_expr_lr true N e1 else None
   (* These two only contain types, therefore Lo *)
   | Esizeof _ _ => Some Lo
   | Ealignof _ _ => Some Lo
   end.
+
+Definition clsf_expr := clsf_expr_lr false.
+Definition clsf_lvalue := clsf_expr_lr true.
