ifc/proofauto_lemmas.v
@@ -62,6 +62,7 @@ Proof.
   - instantiate (1:=
       (fun x => (local (`(eq (v x)) (eval_expr b))) && PROPx (P x) (LOCALx (Q x) (SEPx (R x))))).
     intro. apply andp_right; [ apply (Ev x) | ]. apply andp_left2. apply derives_refl.
+  - admit.
   - unfold pre_assert in *. remember (fun x : T =>
      andp
      ((fun x0 : T =>
